Implement `from_bytes_be`
This puts in place a correct implementation of `from_bytes_be` which
does not defer to `from_bytes_le`.  As such, proving correctness for
this should be straightforward.

src/LeanEVM/Util/Bytes.lean
@@ -20,32 +20,34 @@ def from_bytes_le(bytes:List UInt8) : Nat :=
 -- passed into `from_bytes_le` then the return value is bounded by `256`;
 -- likewise, if two bytes are passed into `from_bytes_le` then the return value
 -- is bounded by `65536`, etc.
-def from_bytes_le_bound(n:Nat)(bytes:List UInt8)(p:bytes.length ≤ n) : (from_bytes_le bytes) < 256^n :=
+def from_bytes_le_bound(bytes:List UInt8) : (from_bytes_le bytes) < 256^bytes.length :=
 by
-  match n,bytes with
-  | 0, [] => unfold from_bytes_le; simp
-  | k+1, [] =>
-      have q : 0 ≤ k := by simp
-      have r : (from_bytes_le []) < 256^k := (by apply from_bytes_le_bound k [] q)
-      have s : 256^k < 256^(k+1) := by apply Nat.pow_lt_pow_succ; simp
-      exact Nat.lt_trans r s
-  | k+1, b::bs =>
-      have q : bs.length ≤ k := by unfold List.length at p; exact Nat.le_of_lt_succ p
-      have r : (from_bytes_le bs) < 256^k := (by apply from_bytes_le_bound k bs q)
-      unfold from_bytes_le
-      apply (pow256_shift (from_bytes_le bs) b k r)
+  match bytes with
+  | [] => simp_arith
+  | b::bs =>
+      apply pow256_shl
+      apply (from_bytes_le_bound bs)
 
+-- Prove correct translation for sequence of length 1.
 example (n:UInt8): (from_bytes_le [n]) = n.val :=
 by
   repeat unfold from_bytes_le
   simp
   rfl
 
+-- Prove correct translation for simple sequence of length 2.
 example (n:UInt8): (from_bytes_le [n, 0]) = n.val :=
 by
   repeat unfold from_bytes_le
   simp
   rfl
+
+-- Prove correct translation for arbitrary sequence of length 2.
+example (m:UInt8)(n:UInt8): (from_bytes_le [m, n]) = m.val + (256*n.val) :=
+by
+  repeat unfold from_bytes_le
+  unfold UInt8.toNat
+  simp_arith
 
 -- ==================================================================================
 -- From Bytes (big endian)
@@ -54,26 +56,41 @@ by
 -- Construct a natural number from a sequence of one or more bytes stored in big
 -- endian form.
 def from_bytes_be(bytes:List UInt8) : Nat :=
-  from_bytes_le (List.reverse bytes)
+  match bytes with
+  | List.nil => 0
+  | b::bs =>
+      let n := bs.length
+      ((256^n) * b.toNat) + (from_bytes_be bs)
 
 -- Bound the number returned by `from_bytes_be`.  For example, if one byte is
 -- passed into `from_bytes_le` then the return value is bounded by `256`;
 -- likewise, if two bytes are passed into `from_bytes_be` then the return value
 -- is bounded by `65536`, etc.
-def from_bytes_be_bound(n:Nat)(bytes:List UInt8)(p:bytes.length ≤ n) : (from_bytes_be bytes) < 256^n :=
+def from_bytes_be_bound(bytes:List UInt8) : (from_bytes_be bytes) < 256^bytes.length :=
 by
-  sorry
+  match bytes with
+  | [] => simp_arith
+  | b::bs =>
+      apply pow256_shr
+      apply (from_bytes_be_bound bs)
 
+-- Prove correct translation for sequence of length 1.
 example (n:UInt8): (from_bytes_be [n]) = n.val :=
 by
-  unfold from_bytes_be
-  repeat unfold from_bytes_le
-  simp
-  rfl
+  repeat unfold from_bytes_be
+  unfold UInt8.toNat
+  simp_arith
 
+-- Prove correct translation for simple sequence of length 2.
 example (n:UInt8): (from_bytes_be [0, n]) = n.val :=
 by
-  unfold from_bytes_be
-  repeat simp; unfold from_bytes_le
+  repeat unfold from_bytes_be
+  unfold UInt8.toNat
+  simp_arith
+
+-- Prove correct translation for arbitrary sequence of length 2.
+example (m:UInt8)(n:UInt8): (from_bytes_be [m, n]) = (256*m.val) + n.val :=
+by
+  repeat unfold from_bytes_be
   unfold UInt8.toNat
   simp_arith
