src/LeanEVM/Util/Lemmas.lean
@@ -7,8 +7,16 @@ by
   exact Nat.mul_le_mul_left m p
 
 -- A simple proof for "left shifting" bytes.  This could no doubt be generalised.
-def pow256_shift(n:Nat)(m:UInt8)(k:Nat)(p:n < 256^k) : (256*n + m.val < 256^(k+1)) :=
+def pow256_shl(n:Nat)(m:UInt8)(k:Nat)(p:n < 256^k) : (256*n + m.val < 256^(k+1)) :=
 by
   have s : 256*n + 256 ≤ 256^(k+1) := (pow_shift n 256 k p)
   have r : 256*n + m.val < 256*n + 256 := by exact Fin.natAdd.proof_1 (256 * n) m.val
   exact Nat.lt_of_lt_of_le r s
+
+-- A simple proof for "right shifting" bytes.  This could no doubt be generalised.
+def pow256_shr(n:Nat)(m:UInt8)(k:Nat)(p:n < 256^k) : (256^k * m.val + n < 256^(k+1)) :=
+by
+  have q1 : n + 255*256*k < (1+255)*256^k := sorry
+  have q2 : n + 255*256*k < 256^k + 255*256^k := by simp at q1; sorry
+  have q3 : n < 256^k := by exact p
+  sorry
